More progress - now can rearrange registers

src/register_machine.lean
@@ -13,12 +13,37 @@ import init.data.nat.basic
 import logic.function.iterate
 
 instance encodable.list {α} [encodable α] : encodable (list α)
-  := ⟨list.rec 0 (λ h _, nat.mkpair (encodable.encode h)),
-      sorry,
-      sorry⟩
+  := ⟨list.rec 0 (λ h _ t', (nat.mkpair (encodable.encode h) t').succ),
+      @nat.strong_rec' (λ _, option (list α)) (λ n,
+        @nat.cases_on (λ n, (Π (m : ℕ), m < n → option (list α)) → option (list α)) n
+          (λ _, some [])
+          (λ n' f,
+            let p := nat.unpair n' in
+            (encodable.decode α p.fst).bind (λ h,
+            (f p.snd begin
+              refine nat.lt_succ_iff.mpr _,
+              exact nat.unpair_le_right n',
+            end).map (λ t, h::t)
+            )
+          )
+      ),
+      begin
+        intro, induction a,
+        simp, dsimp, rw [nat.strong_rec'], simp,
+        simp, dsimp, rw [nat.strong_rec'], simp,
+        convert a_ih, rw nat.unpair_mkpair,
+      end⟩
+
+instance encodable.vector {α} [encodable α] {n} : encodable (vector α n)
+  := encodable.subtype
 
 instance encodable.fin_tuple {n : ℕ} {α : Type*} [encodable α] : encodable (fin n → α)
-  := encodable.of_equiv (list α) sorry
+  := encodable.of_equiv (vector α n)
+      ⟨vector.of_fn, vector.nth,
+        begin intro, ext, exact vector.nth_of_fn x x_1, end,
+        vector.of_fn_nth⟩
+
+notation f `<-[` x `]` y := function.update f x y
 
 namespace rm
 
@@ -26,6 +51,7 @@ namespace rm
     dec r l k  ->  if (r) > 0 then decrement r and jump to l, else jump to k
     jump to halt represented by none instead of a line number
  -/
+@[derive decidable_eq]
 inductive instr (rc ic : ℕ)
 | inc  : fin rc → option (fin ic) → instr
 | dec  : fin rc → option (fin ic) → option (fin ic) → instr
@@ -64,13 +90,39 @@ variables {rc ic : ℕ}
         begin intro, iterate {cases x, simp [equiv_destr._match_1, equiv_destr._match_2]},
               cases x_snd, simp [equiv_destr._match_1, equiv_destr._match_2], end⟩
 
-  instance {rc ic : ℕ} : encodable (instr rc ic)
+  instance encodable {rc ic : ℕ} : encodable (instr rc ic)
     := encodable.of_equiv _ equiv_destr
+
+  instance has_repr {rc ic : ℕ} : has_repr (instr rc ic)
+    := ⟨@instr.rec rc ic (λ _, string)
+        (λ r l,
+          "(rm.instr.inc ".append (
+          (repr r)        .append (
+          " "             .append (
+          (repr l)        .append (
+          ")"
+          ))))
+        ) (λ r l k,
+          "(rm.instr.dec ".append (
+          (repr r)        .append (
+          " "             .append (
+          (repr l)        .append (
+          " "             .append (
+          (repr k)        .append (
+          ")"
+          ))))))
+        )⟩
 
 end instr
 
 /- register machine program with rc registers, ic instructions -/
 @[reducible] def prog (rc ic : ℕ) := fin ic → (instr rc ic)
+@[reducible] def prog' (rc : ℕ) := Σ ic, prog rc ic
+
+namespace prog
+  instance has_repr {rc ic : ℕ} : has_repr (prog rc ic) :=
+    ⟨@repr _ subtype.has_repr ∘ vector.of_fn⟩
+end prog
 
 /- config consists of an instruction pointer and registers. -/
 structure config (rc ic : ℕ) := (ip : option (fin ic)) (regs : fin rc → ℕ)
@@ -111,10 +163,10 @@ namespace prog
     | none := c
     | some ip :=
       match P ip with
-      | instr.inc r l := {ip := l, regs := function.update c.regs r (c.regs r + 1)}
+      | instr.inc r l := {ip := l, regs := c.regs <-[r] (c.regs r + 1)}
       | instr.dec r l k :=
           match c.regs r with
-          | p + 1 := {ip := l, regs := function.update c.regs r p}
+          | p + 1 := {ip := l, regs := c.regs <-[r] p}
           | 0 := {ip := k, regs := c.regs}
           end
       end
@@ -150,7 +202,7 @@ namespace prog
       simpa using h1,
       simpa using h2,
     end
-  
+
   lemma step_t_trans {c d e : config rc ic} {t1 t2 : ℕ}
     (h1 : c [P]==>^[t1] d) (h2 : d [P]==>^[t2] e)
     : c [P]==>^[t1+t2] e
@@ -204,11 +256,10 @@ namespace prog
   theorem eval_mem_iff_steps {rcp ic : ℕ} (P : prog rcp.succ ic) {n m : ℕ}
     : m ∈ P.eval n ↔ ∃ tail, config.init n [P]==>* config.halted (fin.cons m tail)
     := sorry
-
-
+  
 end prog
 
-namespace prog
+namespace progs
   def id : prog 1 0 := ![]
 
   theorem id.behavior (n : ℕ)
@@ -223,57 +274,181 @@ namespace prog
         rw fin.update_cons_zero, refl,
       end
 
-  def embed {rc ic : ℕ} (P : prog rc ic) {rc' : ℕ} (f : fin rc → fin rc')
-    : prog rc' ic
+  section variables {rc rc' ic : ℕ} (P : prog rc ic)
+                    (f : fin rc → fin rc')
+  def embed : prog rc' ic
     := (instr.map_regs f) ∘ P
   
-/-   section
-    variables {rc ic : ℕ} (P : prog rc ic) {rc' : ℕ}
-        (f : fin rc → fin rc')
-        (h : ∀ r', )
+  variable (finv : fin rc' → (fin rc) ⊕ ℕ)
+  @[simp] def embed.reg_map (regs : fin rc → ℕ) : fin rc' → ℕ
+    := λ r', match finv r' with sum.inl r := regs r | sum.inr x := x end
 
-    variables
-      {ip1 ip2 : fin ic} {r1 r2 : fin rc → ℕ}
-      {r1' : fin rc' → ℕ} (h : r1 = r1' ∘ f)
+  @[simp] def embed.config_map (c : config rc ic) : config rc' ic := ⟨c.ip, embed.reg_map finv c.regs⟩
 
-    lemma embed_regs_preserves_step
-      (behav : ⟨ip1, r1⟩ [P]==> ⟨ip2, r2⟩)
-      : ⟨ip1, r1'⟩ [embed P f]==> ⟨ip2, embed_regs_res⟩
-      := begin end
+  variable (h_finv : (∀ r, finv (f r) = sum.inl r) ∧
+              (∀ r', sum.elim (λ r, r' = f r) (λ _, true) (finv r'))
+            )
+  include h_finv
 
-    theorem embed_regs_preserves_behavior
-      (behav : ⟨ip1, r1⟩ [P]==>* ⟨ip2, r2⟩)
-      : ⟨ip1, r1'⟩ [embed P f]==>* ⟨ip2, r2'⟩
+  lemma embed.preserve_step
+    : (embed.config_map finv) ∘ P.step = (embed P f).step ∘ (embed.config_map finv)
+    := begin
+      ext c, simp [embed.reg_map, embed.config_map],
+      cases c with ip regs,
+      cases ip,
+      case none { simp [prog.step] },
+      case some {
+      cases h : P ip with r ip' r ip' ip'',
+      case inc {
+        simp [embed, prog.step, h, embed.config_map],
+        rw h_finv.1 r,
+        ext,
+        cases h2 : finv x,
+        case inr {
+          simp [←h2, function.update],
+          rw h2, simp,
+          have : ¬ x = f r :=
+            begin
+              intro h3,
+              rw h3 at h2,
+              rw h_finv.1 r at h2,
+              simpa using h2,
+            end,
+          simp [this],
+        },
+        case inl {
+          simp [←h2, function.update],
+          rw h2, simp [function.update],
+          congr' 1, ext,
+          have := h_finv.2 x,
+          rw h2 at this, simp at this, rw this,
+          split,
+          intro h, rw h,
+          intro h,
+          have h1 := h_finv.1 val,
+          have h2 := h_finv.1 r,
+          rw [h,h2] at h1,
+          simp at h1, exact h1.symm,
+        }
+      },
+      case dec {
+      cases hr : regs r,
+      case zero {
+        simp [embed, prog.step, h, hr],
+        rw h_finv.1 r,
+        simp [prog.step, hr],
+      },
+      case succ {
+        simp [embed, prog.step, h, hr],
+        rw h_finv.1 r,
+        simp [prog.step, hr],
+        ext,
+        cases h2 : finv x,
+        case inr {
+          simp [←h2, function.update],
+          rw h2, simp,
+          have : ¬ x = f r :=
+            begin
+              intro h3,
+              rw h3 at h2,
+              rw h_finv.1 r at h2,
+              simpa using h2,
+            end,
+          simp [this],
+        },
+        case inl {
+          simp [←h2, function.update],
+          rw h2, simp [function.update],
+          congr' 1, ext,
+          have := h_finv.2 x,
+          rw h2 at this, simp at this, rw this,
+          split,
+          intro h, rw h,
+          intro h,
+          have h1 := h_finv.1 val,
+          have h2 := h_finv.1 r,
+          rw [h,h2] at h1,
+          simp at h1, exact h1.symm,
+        },
+      }}},
+    end
+
+    lemma embed.preserves_steps
+      : ∀ t, (embed.config_map finv) ∘ (P.step^[t]) =
+              ((embed P f).step^[t]) ∘ (embed.config_map finv)
       := begin
-        cases behav, use behav_w,
-        induction behav_w,
-        simp at *, split, exact behav_h.1,
-        
+        intro, induction t,
+        case zero { simp, },
+        case succ : w {
+          rw function.iterate_succ,
+          rw ←function.comp.assoc,
+          rw t_ih,
+          rw function.comp.assoc,
+          rw embed.preserve_step P f finv,
+          refl,
+          exact h_finv,
+        },
       end
-  end -/
 
-  def seq {rc ic1 ic2 : ℕ} (P1 : prog rc ic1) (P2 : prog rc ic2)
-    : prog rc (ic1+ic2) :=
-      fin.append
-        (rfl : ic1+ic2 = ic1+ic2)
-        (instr.map_locs (λ o : option (fin ic1), match o with
+    theorem embed.behavior {ip ip' : option (fin ic)} {regs regs' : fin rc → ℕ}
+      (behav : ⟨ip,regs⟩ [P]==>* ⟨ip',regs'⟩)
+      : ⟨ip, embed.reg_map finv regs⟩ [embed P f]==>*
+          ⟨ip', embed.reg_map finv regs'⟩
+      := begin
+        cases behav with w h,
+        use w,
+        simp,
+        have emps := embed.preserves_steps P f finv h_finv w,
+        have : (embed.config_map finv ∘ (P.step^[w])) ⟨ip,regs⟩ = ((embed P f).step^[w] ∘ embed.config_map finv) ⟨ip,regs⟩,
+          rw emps, clear emps,
+        simp at h,
+        simp [h, embed.config_map] at this,
+        exact this.symm,
+      end
+  end
+
+  section
+    variables {rc ic1 ic2 : ℕ} (P1 : prog rc ic1) (P2 : prog rc ic2)
+    include P1 P2
+
+    def seq.midpoint_ic : option (fin (ic1+ic2))
+      := (config.init_ip rc ic2).map (λ z,
+          ⟨ic1 + z, begin exact nat.add_lt_add_left z.prop ic1, end⟩)
+
+    def seq : prog rc (ic1+ic2) :=
+      fin.append rfl
+        (instr.map_locs (λ o, match o with
                               | some i := some ⟨i.val, i.val.lt_add_right ic1 ic2 i.prop⟩
-                              | none := match ic2 with
-                                        | 0 := none
-                                        | ic2p+1 := some ⟨ic1, nat.add_lt_add_left fin.last_pos ic1⟩
-                                        end
+                              | none := seq.midpoint_ic P1 P2
                               end)
             ∘ P1)
         (instr.map_locs (option.map (λ i, ⟨ic1 + i,nat.add_lt_add_left i.prop ic1⟩))
             ∘ P2)
 
-  lemma seq.behavior {rc ic1 ic2 : ℕ} {P1 : prog rc ic1} {P2 : prog rc ic2}
-    {n : ℕ} {r1 r2 r3 : fin rc → ℕ}
-    (h1 : {ip := config.init_ip rc ic1, regs := r1} [P1]==>* config.halted r2)
-    (h2 : {ip := config.init_ip rc ic2, regs := r2} [P2]==>* config.halted r3)
-    : {ip := config.init_ip rc (ic1+ic2), regs := r1}
-          [seq P1 P2]==>* config.halted r3
-    := sorry
+    def seq' (P1 P2 : prog' rc) : prog' rc :=
+      ⟨P1.fst+P2.fst, seq P1.snd P2.snd⟩
+
+    lemma seq.behavior
+      {r1 r2 r3 : fin rc → ℕ}
+      (h1 : ⟨config.init_ip rc ic1, r1⟩ [P1]==>* config.halted r2)
+      (h2 : ⟨config.init_ip rc ic2, r2⟩ [P2]==>* config.halted r3)
+      : ⟨config.init_ip rc (ic1+ic2), r1⟩ [seq P1 P2]==>* config.halted r3
+      := begin
+        have phase1 : ⟨config.init_ip rc (ic1+ic2), r1⟩ [seq P1 P2]==>* ⟨seq.midpoint_ic P1 P2, r2⟩,
+          cases h1, use h1_w,
+          induction h1_w,
+            simp at h1_h |-, split, swap, exact h1_h.2,
+            simp [seq.midpoint_ic],
+            rw (sorry : ic1 = 0),
+            simp [nat.zero_add, fin.zero_add],
+            exact sorry,
+          exact sorry,
+        have phase2 : ⟨seq.midpoint_ic P1 P2, r2⟩ [seq P1 P2]==>* config.halted r3,
+          exact sorry,
+        exact prog.steps_to_trans (seq P1 P2) phase1 phase2,
+      end
+
+  end
 
   def loop {rc ic : ℕ} (P : prog rc ic)
     : prog rc.succ ic.succ
@@ -298,13 +473,88 @@ namespace prog
       simp,
     end
 
-  def mov {rc : ℕ} (_fr _to : fin rc) : prog rc 2
-    := embed (loop (![instr.inc 0 none])) ![_fr, _to]
+  @[simp] def mov.loop_prog : prog 1 1 := ![instr.inc 0 none]
+  def mov : prog 2 2 := loop (mov.loop_prog)
   
-  theorem mov.behavior {rc ic : ℕ} (_fr _to : fin rc) {hr : _fr ≠ _to}
-    : sorry
-    := sorry
-end prog
+  theorem mov.behavior {n m : ℕ}
+    : ⟨some 0, ![n, m]⟩ [mov]==>* ⟨none, ![0, n+m]⟩
+    := begin have :=
+          loop.behavior mov.loop_prog (λ regs, regs <-[0] (regs 0).succ)
+          (begin intros, use 1, dsimp [prog.step], refl, end) n ![m],
+      convert this, clear this,
+      induction n, simp,
+      rw function.iterate_succ_apply', rw ←n_ih,
+      simp [matrix.vec_cons], rw fin.update_cons_zero, congr,
+      exact nat.succ_add n_n m,
+    end
+
+  @[simp] def dup.loop_prog : prog 2 2 := ![instr.inc 0 (some 1), instr.inc 1 none]
+  lemma dup.loop_prog.behavior (regs : fin 2 → ℕ)
+    : ⟨some 0, regs⟩ [dup.loop_prog]==>* ⟨none, ![(regs 0).succ, (regs 1).succ]⟩
+    := begin
+      use 2, simp [prog.step], ext x, cases x,
+      cases x_val, simp [function.update],
+      simp, cases x_val, simp [function.update],
+      apply false.elim (nat.not_lt_zero x_val _),
+      iterate 2 {
+        apply nat.lt_of_succ_lt_succ _,
+      }, exact x_property,
+    end
+
+  def dup : prog 3 3 := loop (dup.loop_prog)
+  theorem dup.behavior (a b c : ℕ)
+    : ⟨some 0, ![a,b,c]⟩ [dup]==>* ⟨none, ![0, b+a, c+a]⟩
+    := begin have :=
+          loop.behavior dup.loop_prog
+          (λ regs, ![(regs 0).succ, (regs 1).succ])
+          (dup.loop_prog.behavior) a ![b,c],
+      convert this, clear this,
+      induction a, simp,
+      rw function.iterate_succ_apply', rw ←a_ih,
+      simp,
+    end
+
+  def double : prog 3 7 :=
+    cast (by refl) (
+      seq dup (
+        seq
+          (embed mov ![1,0])
+          (embed mov ![2,0])
+      )
+    )
+  
+  section open sum
+  theorem double.behavior (n : ℕ)
+    : config.init n [double]==>* config.halted ![2*n,0,0]
+    := begin
+      have db := dup.behavior n 0 0, simp at db,
+      have h_c1 : ![0,n,n] = embed.reg_map ![inl 1, inl 0, inr n] ![n, 0]
+          := begin ext, fin_cases x, iterate { simp, }, end,
+      rw h_c1 at db,
+      have em1 := embed.behavior mov ![1,0] ![inl 1, inl 0, inr n] (begin 
+          split, intro, fin_cases r, iterate {simp,},
+          intro, fin_cases r', iterate {simp,},
+        end) (@mov.behavior n 0),
+      have h_c2 : embed.reg_map ![inl 1, inl 0, inr n] ![0, n + 0] =
+                  embed.reg_map ![inl 1, inr 0, inl 0] ![n, n]
+          := begin ext, fin_cases x, iterate { simp, }, end,
+      rw h_c2 at em1,
+      have em2 := embed.behavior mov ![2,0] ![inl 1, inr 0, inl 0] (begin 
+          split, intro, fin_cases r, iterate {simp,},
+          intro, fin_cases r', iterate {simp,},
+        end) (@mov.behavior n n),
+      have h_c3 : embed.reg_map ![inl 1, inr 0, inl 0] ![0, n + n] =
+                  ![2*n, 0, 0]
+          := begin ext, fin_cases x, iterate {simp, abel,}, end,
+      rw h_c3 at em2,
+      have s1 := seq.behavior _ _ em1 em2,
+      have s2 := seq.behavior _ _ db s1,
+      convert s2,
+      simp, ext, fin_cases x, iterate { simp, simpa, },
+    end
+  end
+  
+end progs
 
 /- encodable type where an RM can recognize
     valid/invalid encodings (to prevent adding
@@ -321,8 +571,8 @@ namespace rmcodable
   section
     variables {α : Type*} [c : rmcodable α]
 
-    def encode : α → ℕ := c.to_encodable.encode
-    def decode : ℕ → option α := c.to_encodable.decode
+    @[simp] def encode : α → ℕ := c.to_encodable.encode
+    @[simp] def decode : ℕ → option α := c.to_encodable.decode
   end
   
   def of_equiv {β} (α) [c : rmcodable α] (e : β ≃ α) : rmcodable β
@@ -339,9 +589,9 @@ namespace rmcodable
         rw ←this, exact this_h,
       end⟩
   
-  instance nat : rmcodable ℕ := ⟨encodable.nat, prog.succ, begin
+  instance nat : rmcodable ℕ := ⟨encodable.nat, progs.succ, begin
       intros, rw prog.eval_mem_iff_steps, use ![],
-      exact prog.succ.behavior n,
+      exact progs.succ.behavior n,
     end⟩
 
   instance fin (n) : rmcodable (fin n)
@@ -379,10 +629,20 @@ namespace rmcodable
 
 end rmcodable
 
-def apply {rcp ic : ℕ} (P : prog rcp.succ ic)
-    {α β : Type*} [rmcodable α] [rmcodable β] : α →. β
-  := λ a, (P.eval (rmcodable.encode a)).bind
-            (roption.of_option ∘ (@rmcodable.decode β _))
+namespace prog
+  def apply {rcp ic : ℕ} (P : prog rcp.succ ic)
+      {α β : Type*} [rmcodable α] [rmcodable β] : α →. β
+    := λ a, (P.eval (rmcodable.encode a)).bind
+              (roption.of_option ∘ (@rmcodable.decode β _))
+  
+  def add : prog 3 10 := sorry
+  theorem add.behavior : add.apply = pfun.lift (λ pair : ℕ × ℕ, pair.fst + pair.snd)
+    := begin
+      simp [apply, pfun.lift], ext,
+      exact sorry,
+    end
+
+end prog
 
   /- goal: build up this universal machine
 
@@ -399,11 +659,12 @@ def apply {rcp ic : ℕ} (P : prog rcp.succ ic)
   10 := pop I p 2
   11 := dec x 12 12
   12 := write R r x 2
+
   -/
 
 def univ_machine : prog (nat.succ sorry) sorry := sorry
 
 theorem univ_machine_computes_eval {rcp ic : ℕ} (P : prog rcp.succ ic)
-  (n : ℕ) : apply univ_machine (P,n) = P.eval n := sorry
+  (n : ℕ) : prog.apply univ_machine (P,n) = P.eval n := sorry
 
 end rm
